Amend definitions of labeled things. (#1642)
The main reason for this change is to make the proj_node_state_to_proj_n
provable, while still supporting creating/destroying nodes and channels
that are labeled secret.

The main change is that for objects that have labels:
- labels are now decoupled from the rest of the object
- the objects are replaced by options, and empty versions are really
none. This is done with the definition "labeled" in RuntimeModel.v

To give confidence that this change makes forward progress, note that
- secret labeled objects holding a None are indistinguishable from real
ones, so this does not undo the change in
[#1603](https://github.com/project-oak/oak/pull/1603)
- If a nid/handle points to a real object in a projected state, it does
also guarantee the same is true in the non-projected state, making the
troublesome theorem provable.

As a side-effect the definitions of several theorems in NIUtilTheorems
get better reuse, and the low projections are also probably more
trustworthy since they are more clearly distinguished from real objects.

This change does unfortunately break a lot of the proofs.

experimental/ni_coq/vfiles/PossibilisticNI.v
@@ -134,10 +134,12 @@ Hint Extern 4 (state_low_eq _ _ (state_low_proj _ _)) => symmetry : unwind.
 Hint Extern 2 (chan_low_proj _ _ = chan_low_proj _ _)
 => simple eapply chan_low_proj_loweq : unwind.
 
-Hint Extern 4 (_ <<L clbl (chan_low_proj _ _))
+Hint Extern 4 (_ <<L lbl (chan_low_proj _ _))
 => (rewrite chan_projection_preserves_lbl) : flowsto.
 
 Definition is_init(t: trace) := length t = 1.
+
+Definition empty_event (ell: level) := Labeled event None ell.
 
 Definition conjecture_possibilistic_ni := forall ell t1_init t2_init t1n,
     (trace_low_eq ell t1_init t2_init) /\
@@ -148,15 +150,18 @@ Definition conjecture_possibilistic_ni := forall ell t1_init t2_init t1n,
         (step_system_ev_multi t2_init t2n) /\
         (trace_low_eq ell t1n t2n)).
 
-Theorem unobservable_node_step: forall ell s s' e id n,
-    s.(nodes).[? id] = Some n ->
+Theorem unobservable_node_step: forall ell s s' e id nl n,
+    s.(nodes).[? id] = nl ->
+    nl.(obj) = Some n ->
     step_node_ev id n.(ncall) s s' e ->
-    ~(nlbl n <<L ell) ->
-    (state_low_eq ell s s') /\ (event_low_eq ell e (empty_event e.(elbl))).
+    ~(lbl nl <<L ell) ->
+    (state_low_eq ell s s') /\ (event_low_eq ell e (empty_event e.(lbl))).
 Proof.
-    intros. inversion H0; (split; [ inversion H4 | ] ); subst_lets; crush.
+    intros. inversion H1; (split; [ inversion H5 | ] ); subst_lets; crush.
+Admitted.
+(*
     - (* WriteChannel; states loweq *) 
-        assert ( ~ (clbl ch <<L ell) ) by eauto using ord_trans.
+        assert ( ~ (lbl (chans s).[? han] <<L ell) ) by eauto using ord_trans.
         eapply state_low_eq_trans.
         eapply (state_upd_node_unobs _ _ _ _ (node_del_rhans (rhs msg) n)
             ltac:(eauto) ltac:(eauto) ltac:(eauto)).
@@ -222,6 +227,7 @@ Proof.
     unfold event_low_eq. unfold low_eq.
     erewrite event_low_proj_idempotent. reflexivity.
 Qed.
+*)
 
 Theorem step_implies_lowproj_steps_leq: forall ell s1 s1' e1,
     (step_system_ev s1 s1' e1) ->
@@ -232,53 +238,65 @@ Theorem step_implies_lowproj_steps_leq: forall ell s1 s1' e1,
 Proof.
     intros. inversion H; subst. 
     - (* SystemSkip *)
-        exists (state_low_proj ell s1'), (EvL NilEv ell0); repeat try split.
+        exists (state_low_proj ell s1'), (empty_event ell0); repeat try split.
         constructor. symmetry. eapply state_low_proj_loweq.
     - (* NodeSetp *)
         rename s' into s1'. rename s'' into s1''. rename H2 into H_step_s1_s1'.
-        destruct (n.(nlbl) <<? ell).
+        remember ((nodes s1).[?id]) as nl.
+        destruct (nl.(lbl) <<? ell).
         * (* flowsto case *)
-            inversion H_step_s1_s1'; crush; 
-                pose proof (state_nidx_to_proj_state_idx ell _ _ _
+            inversion H_step_s1_s1'; crush; remember ((nodes s1).[?id]) as nl;
+                pose proof (state_nidx_to_proj_state_idx ell _ _ nl
                     ltac:(eauto)) as Hn_idx_s1proj;
-                (rewrite flows_node_proj in *; eauto);
+                (erewrite flows_labeled_proj in Hn_idx_s1proj; eauto);
                 inversion H3; crush.
             + (* WriteChannel *)
-                do 2 eexists; split_ands; [ | | reflexivity ].
+                do 2 eexists; split_ands; [ | | reflexivity ]; admit.
+                (*
                 1:apply_all_constructors;
                   solve [eauto using state_hidx_to_proj_state_hidx with flowsto].
                 subst_lets. eauto 7 with unwind.
+                *)
             + (* ReadChannel *)
+                admit.
+                (*
                 pose proof (state_hidx_to_proj_state_hidx ell _ _ _
                     ltac:(eauto)) as Hch_hidx_s1proj.
                 rewrite flows_chan_proj in *; eauto using ord_trans.
                 do 2 eexists; split_ands; [ | | reflexivity ].
                 1:apply_all_constructors; solve [eauto].
                 subst_lets. eauto with unwind.
+                *)
             + (* CreateChannel *)
-                do 2 eexists; split_ands; [ | | reflexivity ].
+                do 2 eexists; split_ands; [ | | reflexivity ]; admit.
+                (*
                 1:apply_all_constructors;
                   solve [eauto; rewrite ?proj_pres_handle_fresh; eauto].
                 subst_lets. eauto 6 with unwind.
+                *)
             + (* CreateNode *)
-                do 2 eexists; split_ands; [ | | reflexivity ].
+                do 2 eexists; split_ands; [ | | reflexivity ]; admit.
+                (*
                 1:apply_all_constructors;
                   solve [eauto; rewrite ?proj_pres_nid_fresh; eauto].
                 subst_lets. eauto with unwind.
+                *)
             +  (* Internal *)
-                do 2 eexists; split_ands; [ | | reflexivity ].
+                do 2 eexists; split_ands; [ | | reflexivity ]; admit.
+                (*
                 1:apply_all_constructors;
                   solve [eauto; rewrite ?proj_pres_nid_fresh; eauto].
                 subst_lets. eauto with unwind.
+                *)
         * (* not flowsTo case *)
             rename n0 into Hflows.
-            pose proof (unobservable_node_step _ _ _ _ _ _
+            pose proof (unobservable_node_step _ _ _ _ _ nl _ ltac:(eauto)
                 ltac:(eauto) H_step_s1_s1' ltac:(eauto))
                 as [Hustep Huev].
-            exists (state_low_proj ell s1), (empty_event (elbl e1));
+            exists (state_low_proj ell s1), (empty_event (lbl e1));
                 repeat split; crush.
             (* states leq *)
-            pose proof (state_loweq_to_deref_node _ _ _ _ _
+            pose proof (state_loweq_to_deref_node _ _ _ _ (nodes s1).[?id]
                 ltac:(eauto) ltac:(eauto)) 
                 as [ns1' [Hns1'idx Hns1'leq]].
             unfold s1''. transitivity s1'.
@@ -289,7 +307,7 @@ Proof.
             pose proof (state_low_proj_loweq ell s1); congruence.
             (* events leq *)
             congruence.
-Qed.
+Admitted.
 
 Theorem low_proj_steps_implies_leq_step: forall ell s s1' e1,
     (step_system_ev (state_low_proj ell s) s1' e1) ->
@@ -300,21 +318,23 @@ Theorem low_proj_steps_implies_leq_step: forall ell s s1' e1,
 Proof.
     intros. inversion H; subst.
     - (* SystemSkip *)
-        exists s, (EvL NilEv ell0). split. constructor.
+        exists s, (empty_event ell0). split. constructor.
         split. unfold state_low_eq. unfold low_eq.
         rewrite state_low_proj_idempotent. reflexivity.
         reflexivity.
     - (* NodeStep *)
         rename s'' into s1''. rename s' into s1'. rename H2 into H_step_projs_s1'.
-        specialize (proj_node_state_to_proj_n ell s id n H0)
+        remember ((nodes (state_low_proj ell s)).[? id]) as nl.
+        pose proof (uncons_proj_node_s _ _ _ nl ltac:(eauto))
             as [n' [Hidx_n' Hproj_n']].
-        destruct (n'.(nlbl) <<? ell).
+        destruct (nl.(lbl) <<? ell).
         *
-            (* flowsto case*) (* likely by inversion on H_step_projs_s1' *)
-            inversion H_step_projs_s1'; inversion H3;
-                (rewrite flows_node_proj in *; eauto); crush.
-            (* assert (n0 = n) by congruence; subst. *)
-            + (* WriteChannel *)
+            (* flowsto case*)
+            inversion H_step_projs_s1'; inversion H3; 
+                                                (* asterisk doesn't work here anymore? *)
+                (rewrite flows_labeled_proj in Hproj_n'; eauto); crush; admit.
+           (*
+           + (* WriteChannel *)
                 pose proof (uncons_proj_chan_s _ _ _ _ ltac:(eauto))
                     as [ch2 [H_ch'_idx H_ch2_proj]].
                 remember (s_set_call (state_upd_chan han (chan_append ch2 msg)
@@ -362,15 +382,13 @@ Proof.
                 unfold s1''.
                 exists (s_set_call s id c'); eexists; repeat split; crush.
                 eauto with unwind.
+        *)
         (* by cases on the command by n in s *)
         * (* not flowsTo case *)
-            rename n0 into Hflows.
-            assert ((state_low_eq ell (state_low_proj ell s) s1') /\
-                (event_low_eq ell e1 (empty_event e1.(elbl))))
-                as [Hustep Huev] by
-                repeat (eauto || eapply unobservable_node_step
-                    || eapply node_projection_preserves_flowsto).
-            exists s, (empty_event (elbl e1));
+            pose proof (unobservable_node_step _ _ _ _ _ nl _ 
+                ltac:(eauto) ltac:(eauto) ltac:(eauto) ltac:(eauto))
+                as [Hustep Huev].
+            exists s, (empty_event (lbl e1));
                 repeat (split || constructor).
             + (* s1'' ={ell} s *)
                 apply state_low_eq_sym.
@@ -389,11 +407,11 @@ Proof.
                 specialize (state_loweq_to_deref_node ell s s1' id n'
                     Hidx_n' H_leq_s_s1') as [ns1' [Hidx_s1' H_leq_n'_n2]].
                 eapply set_call_unobs. eassumption.
-                replace (nlbl ns1') with (nlbl n')
+                replace (lbl ns1') with (lbl n')
                     by (eapply node_low_eq_to_lbl_eq; eassumption).
-                auto.
+                admit.
             + (* e1 ={ell} *) assumption.
-Qed.
+Admitted.
 
 Theorem possibilistic_ni_1step: forall ell s1 s2 s1' e1,
     (state_low_eq ell s1 s2) ->
