experimental/ni_coq/vfiles/Unwind.v
@@ -32,23 +32,45 @@ Definition state_unwind (f: state -> state):
 but we have to fix the way the definitions are curried.
 *)
 
-Theorem state_upd_node_unwind: forall ell id n1 n2 s1 s2,
+Theorem state_upd_node_unwind: forall ell id n1 n2 n1obj n2obj s1 s2,
+    node_low_eq ell n1 n2 ->
+    n1.(obj) = Some n1obj ->
+    n2.(obj) = Some n2obj ->
+    state_low_eq ell s1 s2 ->
+    state_low_eq ell (state_upd_node id n1obj s1) (state_upd_node id n2obj s2).
+Proof.
+Admitted. (* WIP // TODO *)
+
+Theorem chan_append_unwind: forall ell ch1 ch2 ch1obj ch2obj msg,
+    chan_low_eq ell ch1 ch2 ->
+    ch1.(obj) = Some ch1obj ->
+    ch2.(obj) = Some ch2obj ->
+    chan_low_eq ell 
+        (ch1 <| obj := Some (chan_append ch1obj msg) |>)
+        (ch2 <| obj := Some (chan_append ch2obj msg) |>).
+Proof.
+Admitted. (* WIP // TODO *)
+
+Theorem state_upd_chan_unwind: forall ell han ch1 ch2 ch1obj ch2obj s1 s2,
+    chan_low_eq ell ch1 ch2 ->
+    ch1.(obj) = Some ch1obj ->
+    ch2.(obj) = Some ch2obj ->
+    state_low_eq ell s1 s2 ->
+    state_low_eq ell (state_upd_chan han ch1obj s1) (state_upd_chan han ch2obj s2).
+Proof.
+Admitted.
+
+Theorem state_upd_node_labeled_unwind: forall ell id n1 n2 s1 s2,
     node_low_eq ell n1 n2 ->
     state_low_eq ell s1 s2 ->
-    state_low_eq ell (state_upd_node id n1 s1) (state_upd_node id n2 s2).
+    state_low_eq ell (state_upd_node_labeled id n1 s1) (state_upd_node_labeled id n2 s2).
 Proof.
-Admitted. (* WIP // TODO *)
+Admitted.
 
-Theorem chan_append_unwind: forall ell ch1 ch2 msg,
-    chan_low_eq ell ch1 ch2 ->
-    chan_low_eq ell (chan_append ch1 msg) (chan_append ch2 msg).
-Proof.
-Admitted. (* WIP // TODO *)
-
-Theorem state_upd_chan_unwind: forall ell han ch1 ch2 s1 s2,
+Theorem state_upd_chan_labeled_unwind: forall ell id ch1 ch2 s1 s2,
     chan_low_eq ell ch1 ch2 ->
     state_low_eq ell s1 s2 ->
-    state_low_eq ell (state_upd_chan han ch1 s1) (state_upd_chan han ch2 s2).
+    state_low_eq ell (state_upd_chan_labeled id ch1 s1) (state_upd_chan_labeled id ch2 s2).
 Proof.
 Admitted.
 
@@ -59,38 +81,10 @@ Proof.
     intros. inversion H; subst.
     unfold s_set_call.
     destruct (s1.(nodes).[? id]) eqn:E1; destruct (s2.(nodes).[? id]) eqn:E2.
-    - (* some, some *)
-        assert (E: node_low_eq ell 
-            (n <| ncall ::= (fun x=> c) |>)
-            (n0 <| ncall ::= (fun x=> c) |>)).
-        {
-            admit.
-            (*
-            specialize (H0 id). rewrite E1 in H0.
-            rewrite E2 in H0.
-            inversion H0; subst. 
-            constructor; reflexivity.
-            constructor 2; assumption.
-            *)
-        }
-        eapply state_upd_node_unwind; assumption.
-    - (* some, none *)
-        admit.
-        (*
-        exfalso. specialize (H0 id).
-        rewrite E1, E2 in H0.
-        assumption.
-        *)
-    - (* none, some *)
-        admit.
-        (*
-        exfalso. specialize (H0 id).
-        rewrite E1, E2 in H0.
-        assumption.
-        *)
-    - admit. (* split; assumption *)
 Admitted.
 
 Hint Resolve state_upd_chan_unwind chan_append_unwind
                 set_call_unwind state_upd_node_unwind
-                chan_low_proj_loweq state_low_proj_loweq : unwind.
+                state_upd_chan_labeled_unwind
+                state_upd_node_labeled_unwind
+                labeled_low_proj_loweq : unwind.
